quicstream interface

src/tls/QUICStream.fsti
@@ -34,41 +34,27 @@ val plain_repr : i:I.id{~(AEAD.safeId i)} -> l:plainLen -> p:plain i l -> b:lbyt
 
 type cipher (i:I.id) (l:plainLen) = lbytes (l + v AEAD.taglen)
 
-let max_ctr = pow2 32 - 1
+let max_ctr = pow2 62 - 1
 
-type npn_length =
-  | OneByte
-  | TwoBytes
-  | FourBytes
+let pnlen = n:nat{n=1 \/ n=2 \/ n=4}
 
-let pnlen = PNE.pnlen
-
-let pnlen_of_npn_length (l:npn_length) : pnlen =
-  match l with
-    | OneByte -> 1
-    | TwoBytes -> 2
-    | FourBytes -> 4
-
-val npn: j:I.id -> l:pnlen -> t:Type0{hasEq t}
+(*val npn: j:I.id -> l:pnlen -> t:Type0{hasEq t}
 
 val npn_as_bytes : j:I.id -> l:pnlen -> n:npn j l -> GTot (lbytes l)
 
 val mk_npn: j:I.id -> l:pnlen -> b:lbytes l -> n:npn j l{~(PNE.safePNE j) ==> npn_as_bytes j l n == b}
 
 val npn_repr : j:I.id{~(PNE.safePNE j)} -> l:pnlen -> n:npn j l -> b:lbytes l{b == npn_as_bytes j l n}
-
+*)
 let epn = PNE.epn
 
-let npn_as_nat (j:I.id) (l:pnlen) (n:npn j l) : GTot (m:nat{m < pow2 (Mul.op_Star 8 l)}) =
-  int_of_bytes (npn_as_bytes j l n)
-
-type rpn = n:U64.t{U64.v n <= pow2 62 - 1}
+type rpn = n:U64.t{U64.v n <= max_ctr}
 
 let rpn_of_u32 (j:U32.t) : rpn =
   let jj:nat = U32.v j in
   U64.uint_to_t jj
 
-val npn_of_rpn : (j:I.id) -> (r:rpn) -> (l:pnlen) -> (n:npn j l)
+//val npn_of_rpn : (j:I.id) -> (r:rpn) -> (l:pnlen) -> (n:npn j l)
 
 type stream_entry (i:I.id) (j:I.id) =
   | Entry:
@@ -89,38 +75,58 @@ val invariant: #i:I.id -> #j:I.id -> w:stream_writer i j -> mem -> Type0
 val rinvariant: #i:I.id -> #j:I.id -> #w:stream_writer i j -> r:stream_reader w -> h:mem -> Type0
 
 val wctrT: #i:I.id -> #j:I.id -> w:stream_writer i j -> mem -> GTot (n:nat{n<=max_ctr})
-val wctr: #i:I.id -> #j:I.id -> w:stream_writer i j -> ST UInt32.t
+val wctr: #i:I.id -> #j:I.id -> w:stream_writer i j -> ST rpn
   (requires fun h0 -> True)
-  (ensures fun h0 c h1 -> h0 == h1 /\ UInt32.v c = wctrT w h1)
+  (ensures fun h0 c h1 -> h0 == h1 /\ UInt64.v c = wctrT w h1)
 
-val pnlogT: #i:I.id -> #j:I.id -> #w: stream_writer i j -> r:stream_reader w -> h:mem ->
-  GTot (s:Seq.seq rpn{rinvariant r h /\ safeId i ==> (forall (k:pn j). Seq.mem k s ==> pn_as_nat j k <= wctrT w h)})
+
+val pnlog: #i:I.id -> #j:I.id -> #w: stream_writer i j -> r:stream_reader w -> h:mem ->
+  GTot (s:Seq.seq rpn{rinvariant r h /\ safeId i ==> (forall (k:rpn). Seq.mem k s ==> U64.v k <= wctrT w h)})
   
-val pnlog: #i:I.id -> #j:I.id -> #w: stream_writer i j -> r:stream_reader w -> ST (Seq.seq (pn j))
-  (requires fun h0 -> True)
-  (ensures fun h0 s h1 -> h0 == h1 /\ s == pnlogT r h0)
-
 val wlog: #i:safeid -> #j:I.id -> w:stream_writer i j -> h:mem{invariant w h} -> GTot (s:Seq.seq (stream_entry i j)
   {wctrT w h == Seq.length s})
 
-let pn_filter (i:I.id) (j:I.id) (ns:Seq.seq (pn j)) (e:stream_entry i j) : bool =
+val highest_pnT: #i:I.id -> #j:I.id -> #w:stream_writer i j -> r:stream_reader w -> h:mem ->
+  Ghost (option nat)
+  (requires True)
+  (ensures fun o ->  
+    Some? o ==> 
+    (let n:nat = Some?.v o in
+      n<=max_ctr /\ 
+      (rinvariant r h ==> 
+        (Seq.mem (U64.uint_to_t n) (pnlog r h) /\
+        (forall (k:rpn). Seq.mem k (pnlog r h) ==> U64.v k <= n)))))
+        
+let map_option (#t:Type) (#t':Type) (f:t -> t') (o:option t) :
+  Tot (o':option t') //{(None? o ==> None? o') /\ (Some? o ==> o' == Some (f (Some?.v o)))})
+=
+  match o with
+    | None -> None
+    | Some x -> Some (f x)
+    
+#reset-options "--z3rlimit 50"
+
+val highest_pn: #i:I.id -> #j:I.id -> #w:stream_writer i j -> r:stream_reader w -> ST (option rpn)
+  (requires fun h0 -> True)
+  (ensures fun h0 c h1 -> h0 == h1 /\
+    (highest_pnT #i #j #w r h0 = map_option #rpn #nat U64.v c))
+
+let pn_filter (i:I.id) (j:I.id) (ns:Seq.seq rpn) (e:stream_entry i j) : bool =
   let n = Entry?.pn e in
   Seq.mem n ns
 
-let epn_filter (i:I.id) (j:I.id) (ne:epn) (e:stream_entry i j) : bool =
-  Entry?.ne e = ne
+let epn_filter (i:I.id) (j:I.id) (l:pnlen) (ne:epn l) (e:stream_entry i j) : bool =
+  Entry?.nl e = l && Entry?.ne e = ne
   
 let seq_filter (#a:Type) (f:a -> bool) (s:Seq.seq a) : Seq.seq a =
   Seq.seq_of_list #a (List.Tot.filter #a f (Seq.seq_to_list #a s))
 
-let log_filter (#i:safeid) (#j:I.id) (w:stream_writer i j) (h:mem{invariant w h}) (ns:Seq.seq (pn j)) =
+let log_filter (#i:safeid) (#j:I.id) (w:stream_writer i j) (h:mem{invariant w h}) (ns:Seq.seq rpn) =
   seq_filter (pn_filter i j ns) (wlog w h)
 
 val rlog: #i:safeid -> #j:I.id -> #w:stream_writer i j -> r:stream_reader w -> h:mem{invariant w h /\ rinvariant r h} ->
   GTot (s:Seq.seq (stream_entry i j)
-    {s == log_filter w h (pnlogT r h)})
-
-
+    {s == log_filter w h (pnlog r h)})
 
 let wincrementable (#i:I.id) (#j:I.id) (w:stream_writer i j) (h:mem) =
   wctrT w h < max_ctr
@@ -171,13 +177,23 @@ val frame_log: #i:safeid -> #j:I.id -> w:stream_writer i j -> l:Seq.seq (stream_
   Lemma
   (requires
     Flag.safeId i /\
-    invariant w h0 ->
+    invariant w h0 /\
     wlog w h0 == l /\
     modifies_one ri h0 h1 /\
     ~(Set.mem ri (footprint w)) /\
     ~(Set.mem ri (shared_footprint w)))
   (ensures invariant w h1 ==> wlog w h1 == l)
 
+val frame_pnlog: #i:safeid -> #j:I.id -> #w:stream_writer i j -> r:stream_reader w -> l:Seq.seq rpn ->
+  h0:mem -> ri:rid -> h1:mem ->
+  Lemma
+  (requires
+    Flag.safeId i /\
+    pnlog r h0 == l /\
+    modifies_one ri h0 h1 /\
+    ~(Set.mem ri (rfootprint r)) /\
+    ~(Set.mem ri (shared_footprint w)))
+  (ensures pnlog r h1 == l)
 
 val create: i:I.id -> j:I.id -> u:info i j ->
   ST (stream_writer i j)
@@ -213,7 +229,8 @@ val createReader: parent:rgn -> #i:I.id -> #j:I.id -> w:stream_writer i j ->
     modifies_none h0 h1 /\
     Flag.safeId i ==>
       (rlog r h1 == Seq.empty /\
-      pnlogT r h1 == Seq.empty)
+      pnlog r h1 == Seq.empty /\
+      highest_pnT r h1 == None)
   )
 
 
@@ -235,7 +252,8 @@ val encrypt
     invariant w h1 /\
     wctrT w h1 == wctrT w h0 + 1 /\ 
     (Flag.safeId i ==> (
-      exists (n:pn j nl). (wlog w h1 == Seq.snoc (wlog w h0) (Entry n ad p ne c) /\ wctrT w h0 == pn_as_nat j n))) /\
+      let n = U64.uint_to_t (wctrT w h0) in
+      wlog w h1 == Seq.snoc (wlog w h0) (Entry nl n ad p ne c))) /\
     modifies (Set.union (footprint w) (shared_footprint w)) h0 h1)
 
 //val adata_of_entry: #i:I.id -> stream_entry i -> GTot AEAD.adata
@@ -253,7 +271,8 @@ val decrypt
   (#w:stream_writer i j)
   (r:stream_reader w)
   (ad:AEAD.adata)
-  (ne:epn)
+  (#nl:pnlen)
+  (ne:epn nl)
   (l:plainLen)
   (c:cipher i l):
   ST (option (plain i l))
@@ -261,13 +280,13 @@ val decrypt
   (ensures fun h0 res h1 ->
     rinvariant r h1 /\
     modifies (Set.union (rfootprint r) (rshared_footprint r)) h0 h1 /\
-    (None? res ==> pnlogT r h1 == pnlogT r h0) /\
+    (None? res ==> pnlog r h1 == pnlog r h0) /\
     (Flag.safeId i ==> (
       let lg = wlog w h0 in
-      match (Seq.find_l (epn_filter i j ne) lg) with
+      match (Seq.find_l (epn_filter i j nl ne) lg) with
         | None -> res = None
-        | Some (Entry pn ad' #l' p _ c') ->
-          if ad' = ad && l' = l && c' = c then
-            (res = Some p /\ pnlogT r h1 == Seq.snoc (pnlogT r h0) pn)
+        | Some (Entry nl' pn ad' #l' p _ c') ->
+          if nl = nl' && ad' = ad && l' = l && c' = c then
+            (res = Some p /\ pnlog r h1 == Seq.snoc (pnlog r h0) pn)
           else
             res = None)))
